Add gcd example, showing bug (in elaboration of gcd_unfold probably because the unfolding equation can't be proved).

test-suite/f91.v
@@ -18,7 +18,7 @@ Instance gt_bound_wf : WellFounded f91_rel.
 Proof. red. red. intros.
   Admitted.
 
-Equations(noind) f91 n : { m : nat | if le_lt_dec n 100 then m = 91 else m = n - 10 } :=
+Equations f91 n : { m : nat | if le_lt_dec n 100 then m = 91 else m = n - 10 } :=
 f91 n by rec n f91_rel :=
 f91 n with le_lt_dec n 100 := {
   | left H := exist _ (proj1_sig (f91 (proj1_sig (f91 (n + 11))))) _ ;
@@ -40,19 +40,16 @@ Next Obligation. destruct le_lt_dec. intros. destruct_call f91_comp_proj. simpl.
 Qed.
 
 Next Obligation. destruct le_lt_dec. intros. omega. omega. Defined.
+Solve Obligations.
 
-Obligation Tactic := idtac.
+(** MS: Bug, this should be derivable, but needs the user's proofs as hints (omega calls) *)
+Next Obligation.
+Proof. intros.
+  rec_wf_rel n IH f91_rel.
+  simp f91. constructor. destruct le_lt_dec. constructor. intros. apply IH.
+  do 2 red; omega.
+  apply IH. do 2 red. destruct_call f91. simpl proj1_sig.
+  destruct le_lt_dec; subst; omega.
+  constructor. 
+Defined.
 
-Next Obligation. intro. apply prog. Defined.
-
-(* Next Obligation.  *)
-(* Proof. intros. *)
-(*   rec_wf_rel n IH f91_rel. *)
-(*   simp f91. constructor. destruct le_lt_dec. constructor. intros. apply IH. *)
-(*   do 2 red; omega. *)
-(*   apply IH. do 2 red; omega. *)
-(*   apply IH. do 2 red. destruct_call f91. simpl proj1_sig.  *)
-(*   destruct le_lt_dec; subst; omega. *)
-(*   apply IH. *)
-(*   simp f91. *)
-(* Defined. *)
