test-suite/gcd.v
@@ -1,0 +1,103 @@
+Require Import Equations.
+Require Import Relations.
+
+Definition gcd_order (p : nat * nat) : nat := let (x,y) := p in x+y.
+
+
+Definition measure {A B} (f : A -> B) (R : relation B) : relation A :=
+  fun x y => R (f x) (f y).
+
+Definition gcd_rel : relation (nat * nat) :=
+  MR lt gcd_order.
+
+Instance gt_bound_wf : WellFounded gcd_rel.
+Proof. red. apply measure_wf. apply Wf_nat.lt_wf. Defined.
+
+Require Import Omega.
+
+Hint Extern 5 => 
+  unfold gcd_rel, gcd_order, MR; omega : Below.
+
+Equations gcd (p : nat * nat) : nat :=
+gcd p by rec p gcd_rel :=
+gcd (pair 0 _) := 0 ;
+gcd (pair _ 0) := 0 ;
+gcd (pair x y) with gt_eq_gt_dec x y := {
+  | inleft (left ygtx) := gcd (x, y - x) ;
+  | inleft (right refl) := x ;
+  | inright xgty := gcd (x - y, y) }.
+
+Require Import Utf8.
+Lemma FixF_eq A (R : A -> A -> Prop) P (F : (∀ x : A, (∀ y : A, R y x → P y) → P x)) t step step' : 
+  @Fix_F A R P F t (Acc_intro t step) =
+  F t (fun y rel => @Fix_F A R P F y (step' y rel)).
+Proof. simpl. apply f_equal. extensionality y; extensionality h. 
+       apply f_equal. apply proof_irrelevance.
+Defined.
+
+Lemma FixWf_eq A (R : A -> A -> Prop) wfr P (F : (∀ x : A, (∀ y : A, R y x → P y) → P x)) t : 
+  @FixWf A R wfr P F t =
+  F t (fun y rel => @FixWf A R wfr P F y).
+Proof. unfold FixWf, Fix. unfold wellfounded.        
+       destruct (wfr t). apply FixF_eq.
+Defined.
+Obligation Tactic := idtac.
+Next Obligation. (*MS: Bug *) intros. admit. Defined.
+
+(*   intros. *)
+(*   rec_wf_rel p IH gcd_rel. *)
+(*   setoid_rewrite FixWf_eq.  *)
+(*   change ( gcd_obligation_8 x *)
+(*      (λ (y : nat * nat) (_ : gcd_rel y x), gcd y) = gcd_unfold x). *)
+(*   Opaque gcd. *)
+(*   depelim x. depelim n. reflexivity. *)
+(*   depelim n0. reflexivity. *)
+(*   simpl. simpl_equations.  *)
+(*   simpl. *)
+(*   destruct_call gt_eq_gt_dec. destruct s. *)
+(*   simpl. simpl. unfold gcd_comp_proj. unfold gcd_obligation_1. *)
+
+(*   autounfold with gcd. specialize (IH (S n, n - n)). *)
+(*   symmetry. rewrite IH. Focus 2. do 3 red; unfold gcd_order. omega.  *)
+(*   unfold gcd_comp_proj. *)
+(*   Transparent gcd gcd_unfold. apply IH. *)
+(* Solve Obligations.  *)
+Next Obligation. 
+  intros. 
+  eapply (@gcd_ind_mut P P0); eauto. 
+  apply gcd_ind_fun.
+Defined.
+
+Lemma gcd_ref x : gcd (x,x) = x.
+Proof.
+  funelim (gcd (x, x)); now (try (exfalso; omega)). 
+Qed.
+
+Module Function.    
+Require Import Recdef.
+Function gcd (p : nat * nat) {measure gcd_order p} : nat :=
+ match p with
+   | (0,_) => 0
+   | (_,0) => 0
+   | (x,y) => match gt_eq_gt_dec x y with
+                | inleft (left _) => gcd (x, y-x)
+                | inleft (right _) => x
+                | inright xgty => gcd (x-y, y)
+              end
+ end.
+- unfold gcd_order ; intros ; omega.
+- unfold gcd_order ; intros ; omega.
+Defined.
+
+Lemma gcd_ref x : gcd (x,x) = x.
+Proof.
+  functional induction (gcd (x, x)). Abort.
+
+Lemma gcd_ref x : gcd (x,x) = x.
+Proof.
+  generalize (@eq_refl _ (x, x)).
+  generalize (x, x) at 1 3. intros p; revert x.
+  functional induction (gcd p); intros; noconf H.
+  red in _x. omega. omega.
+Qed.
+End Function.
